extraction: List length call rule + progress on more complex example

src/CertifiedExtraction/Benchmarks/MicroEncoders.v
@@ -1,39 +1,36 @@
 Require Import Benchmarks.MicroEncodersSetup.
 
-Record FourWords :=
-  { w0 : BoundedNat 8;
-    w1 : BoundedNat 8;
-    w2 : BoundedNat 8;
-    w3 : BoundedNat 8 }.
+(* FIXME why isn't the require export in MicroEncodersSetup working? *)
+Require Export
+        Fiat.Common.SumType
+        Fiat.Common.EnumType
+        Fiat.Common.BoundedLookup
+        Fiat.Common.ilist
+        Fiat.Computation
+        Fiat.BinEncoders.Env.Automation.SolverOpt
+        Fiat.BinEncoders.Env.BinLib.Bool
+        Fiat.BinEncoders.Env.BinLib.Core
+        Fiat.BinEncoders.Env.BinLib.Enum
+        Fiat.BinEncoders.Env.BinLib.FixInt
+        Fiat.BinEncoders.Env.Common.Compose
+        Fiat.BinEncoders.Env.Common.ComposeCheckSum
+        Fiat.BinEncoders.Env.Common.ComposeIf
+        Fiat.BinEncoders.Env.Common.Specs
+        Fiat.BinEncoders.Env.Common.WordFacts
+        Fiat.BinEncoders.Env.Lib.FixList
+        Fiat.BinEncoders.Env.Lib.IList
+        Fiat.BinEncoders.Env.Lib2.Bool
+        Fiat.BinEncoders.Env.Lib2.EnumOpt
+        Fiat.BinEncoders.Env.Lib2.FixListOpt
+        Fiat.BinEncoders.Env.Lib2.NatOpt
+        Fiat.BinEncoders.Env.Lib2.NoCache
+        Fiat.BinEncoders.Env.Lib2.SumTypeOpt
+        Fiat.BinEncoders.Env.Lib2.Vector
+        Fiat.BinEncoders.Env.Lib2.WordOpt
+        Fiat.BinEncoders.Env.Lib2.IPChecksum.
 
 Notation "x 'ThenC' y" := (compose _ x y).
 Notation "x 'DoneC'"   := (x ThenC fun e => (transform_id, e)).
-
-Definition ListOfNat_encode (ls : BoundedList (BoundedNat 8) 256) :=
-  fst (((encode_word_Impl WO~0~0~1~0~1~0~1~0) ThenC
-        (encode_nat_Impl 8 (length (projT1 ls))) ThenC
-        (encode_list_Impl (fun n : BoundedNat _ => encode_nat_Impl 8 (projT1 n)) (projT1 ls))) tt).
-
-Definition FourWords_encode (t : FourWords) :=
-byteString
-  (fst ( ((EncodeBoundedNat t.(w0)
-   ThenC EncodeBoundedNat t.(w1)
-   ThenC EncodeBoundedNat t.(w2)
-   ThenC EncodeBoundedNat t.(w3)
-  DoneC) ()))) : list byte.
-
-(* Open Scope binencoders_scope. *)
-
-Definition FourWordsAsCollectionOfVariables
-  {av} vw0 vw1 vw2 vw3 t
-  : Telescope av :=
-  [[ vw0 ->> t.(w0) as _ ]] ::
-  [[ vw1 ->> t.(w1) as _ ]] ::
-  [[ vw2 ->> t.(w2) as _ ]] ::
-  [[ vw3 ->> t.(w3) as _ ]] :: Nil.
-
-Hint Unfold FourWords_encode : f2f_binencoders_autorewrite_db.
-Hint Unfold FourWordsAsCollectionOfVariables : f2f_binencoders_autorewrite_db.
 
 Open Scope list_scope.
 
@@ -65,8 +62,6 @@ Ltac _compile_decide_AllocString_size :=
     unify x (natToWord sz zz); reflexivity
   end.
 
-Open Scope nat_scope.
-
 Ltac _compile_decide_write8_side_condition :=
   repeat lazymatch goal with
          | [ H := _ |- _ ] => unfold H in *; clear H
@@ -83,7 +78,7 @@ Ltac _compile_encode_do_side_conditions :=
   match goal with
   | [  |- _ = _ ^* _ ] => _compile_decide_AllocString_size
   | [  |- padding _ = 0 ] => _compile_decide_padding_0
-  | [  |- List.length (byteString (?x)) + 1 <= _ ] => _compile_decide_write8_side_condition
+  | [  |- (List.length (byteString (?x)) + 1 <= _)%nat ] => _compile_decide_write8_side_condition
   end.
 
 Ltac compile_encoder_step ::=
@@ -107,6 +102,32 @@ Ltac compile_encoder_step ::=
    | _ => _compile_step
    end.
 
+
+Record FourWords :=
+  { w0 : BoundedNat 8;
+    w1 : BoundedNat 8;
+    w2 : BoundedNat 8;
+    w3 : BoundedNat 8 }.
+
+Definition FourWords_encode (t : FourWords) :=
+byteString
+  (fst ( ((EncodeBoundedNat t.(w0)
+   ThenC EncodeBoundedNat t.(w1)
+   ThenC EncodeBoundedNat t.(w2)
+   ThenC EncodeBoundedNat t.(w3)
+  DoneC) ()))) : list byte.
+
+Definition FourWordsAsCollectionOfVariables
+  {av} vw0 vw1 vw2 vw3 t
+  : Telescope av :=
+  [[ vw0 ->> t.(w0) as _ ]] ::
+  [[ vw1 ->> t.(w1) as _ ]] ::
+  [[ vw2 ->> t.(w2) as _ ]] ::
+  [[ vw3 ->> t.(w3) as _ ]] :: Nil.
+
+Hint Unfold FourWords_encode : f2f_binencoders_autorewrite_db.
+Hint Unfold FourWordsAsCollectionOfVariables : f2f_binencoders_autorewrite_db.
+
 Example FourWords_compile :
   let wrapper := @WrapListByte (natToWord _ 512) in
   ParametricExtraction
@@ -116,19 +137,421 @@ Example FourWords_compile :
                   (NTSome "w0") (NTSome "w1") (NTSome "w2") (NTSome "w3") fourWords)
     #env       MicroEncoders_Env.
 Proof.
-  intros.
-  unfold FourWords_encode.
   Time compile_encoder_t.
   repeat (apply CompileDeallocSCA_discretely; try compile_encoder_t).
-  (* FIXME use these only in the microbenchmarks *)
-  Ltac _compile_mutation ::= fail.
-  Ltac _compile_constructor ::= fail.
-  Ltac _compile_destructor ::= fail.
 Defined.
 
 Eval lazy in (extract_facade FourWords_compile).
 
 Print Assumptions FourWords_compile.
+
+Definition BoundedListLength {A size} (ls : BoundedList A (pow2 size)) : BoundedNat size :=
+  exist _ (length (` ls)) (proj2_sig ls).
+
+Lemma map_inj {A B}:
+  forall (f: A -> B),
+    (forall x y, f x = f y -> x = y) ->
+    (forall x y, (map f) x = (map f) y -> x = y).
+Proof.
+  induction x; destruct y; simpl; intros HH; try congruence.
+  inversion' HH; f_equal; eauto.
+Qed.
+
+Instance WrapList {A B} {Wrp: FacadeWrapper A B} : FacadeWrapper (list A) (list B).
+Proof.
+  refine {| wrap x := map wrap x |}.
+  abstract (eauto using map_inj, wrap_inj).
+Defined.
+
+Lemma WrapBoundedList_inj_1:
+  forall (B : Type) (size : nat) (v v' : BoundedList B size), ` v = ` v' -> v = v'.
+Proof.
+  intros.
+  apply exist_irrel'.
+  - intros; apply lt_uniqueness_proof.
+  - eassumption.
+Qed.
+
+Lemma WrapBoundedList_inj {A B : Type} {size : nat} {Wrp : FacadeWrapper A (list B)}:
+  forall (v v' : BoundedList B size),
+    wrap (` v) = wrap (` v') ->
+    v = v'.
+Proof.
+  intros * H; apply wrap_inj, WrapBoundedList_inj_1 in H; assumption.
+Qed.
+
+Lemma WrapTransitive {A A' A''}
+      {WrpVal: FacadeWrapper A A'}
+      {WrpList: FacadeWrapper A' A''}
+  : FacadeWrapper A A''.
+Proof.
+  refine {| wrap a'' := wrap (wrap a'');
+            wrap_inj := _ |}.
+  abstract (intros * H; repeat apply wrap_inj in H; assumption).
+Defined.
+
+Instance WrapBoundedList {A B size} {Wrp: FacadeWrapper A (list B)} : FacadeWrapper A (BoundedList B size) :=
+  {| wrap bl := wrap (`bl);
+     wrap_inj := WrapBoundedList_inj |}.
+
+Typeclasses eauto := 10.
+
+Instance WrapWordList : FacadeWrapper ADTValue (list W).
+Proof.
+  refine {| wrap tl := WordList tl;
+            wrap_inj := _ |}; abstract (inversion 1; reflexivity).
+Defined.
+
+Instance WrapBoundedListOfBoundedNat {sl} : FacadeWrapper (Value ADTValue) (BoundedList (BoundedNat 8) sl).
+Proof.
+  eapply @WrapTransitive.
+  - apply @WrapInstance.
+    apply @WrapWordList.
+  - apply @WrapBoundedList.
+    apply @WrapList.
+    apply @WrapNatIntoW8.
+Defined.
+
+Eval compute in WrapBoundedListOfBoundedNat.
+
+Record MixedRecord :=
+  { f1 : byte;
+    f2 : BoundedNat 8;
+    f3 : BoundedList (BoundedNat 8) (pow2 8) }.
+
+Definition MixedRecord_encode (mr: MixedRecord) :=
+  byteString
+    (fst (((encode_word_Impl WO~0~0~1~0~1~0~1~0)
+     ThenC (encode_word_Impl mr.(f1))
+     ThenC (EncodeBoundedNat mr.(f2))
+     ThenC (EncodeBoundedNat (BoundedListLength mr.(f3)))
+     ThenC (encode_list_Impl EncodeBoundedNat (projT1 mr.(f3)))) tt)) : list byte.
+
+Definition MixedRecordAsCollectionOfVariables
+  {av} vf1 vf2 vf3 ll : Telescope av :=
+  [[ vf1 ->> ll.(f1) as _ ]] ::
+  [[ vf2 ->> ll.(f2) as _ ]] ::
+  [[ vf3 ->> ll.(f3) as _ ]] :: Nil.
+
+Hint Unfold MixedRecord_encode : f2f_binencoders_autorewrite_db.
+Hint Unfold MixedRecordAsCollectionOfVariables : f2f_binencoders_autorewrite_db.
+
+Example MixedRecord_compile :
+  let wrapper := @WrapListByte (natToWord _ 512) in
+  ParametricExtraction
+    #vars      mixedRecord
+    #program   ret (MixedRecord_encode mixedRecord)
+    #arguments (MixedRecordAsCollectionOfVariables
+                  (NTSome "f1") (NTSome "f2") (NTSome "f3") mixedRecord)
+    #env       MicroEncoders_Env.
+Proof.
+  compile_encoder_step.
+  compile_encoder_step.
+  compile_encoder_step.
+  compile_encoder_step.
+  compile_encoder_step.
+  compile_encoder_step.
+  compile_encoder_step.
+  compile_encoder_step.
+  compile_encoder_step.
+  compile_encoder_step.
+  compile_encoder_step.
+  compile_encoder_step.
+  compile_encoder_step.
+  2:compile_encoder_step.
+  compile_encoder_step.
+  compile_encoder_step.
+  compile_encoder_step.
+  compile_encoder_step.
+  compile_encoder_step.
+  compile_encoder_step.
+  compile_encoder_step.
+  compile_encoder_step.
+  compile_encoder_step.
+  compile_encoder_step.
+  compile_encoder_step.
+  compile_encoder_step.
+  compile_encoder_step.
+  compile_encoder_step.
+  compile_encoder_step.
+  compile_encoder_step.
+  compile_encoder_step.
+  compile_encoder_step.
+  compile_encoder_step.
+  compile_encoder_step.
+  compile_encoder_step.
+
+  Lemma encode_byte_simplify : (* {cache} {cacheAddNat : CacheAdd cache nat} : *)
+    forall (w: byte), (* (c: @CacheEncode cache), *)
+      encode_word_Impl w tt =
+      ({| padding := 0; front := WO; paddingOK := Lt.lt_0_Sn 7; byteString := w :: nil |}, addE tt 8).
+  Proof.
+    unfold encode_word_Impl; intros.
+    rewrite encode_char'; reflexivity.
+  Qed.
+
+  rewrite encode_byte_simplify.
+
+  compile_encoder_step.
+  compile_encoder_step.
+  compile_encoder_step.
+  compile_encoder_step.
+  compile_encoder_step.
+  compile_encoder_step.
+  compile_encoder_step.
+  Focus 3.
+  compile_encoder_step.
+  compile_encoder_step.
+  compile_encoder_step.
+  compile_encoder_step.
+  compile_encoder_step.
+
+  Lemma CompileConstant_SCA:
+    forall {av A} {Wr: FacadeWrapper (Value av) A}
+      name env (w: A) ext (tenv: Telescope av),
+      name ∉ ext ->
+      NotInTelescope name tenv ->
+      (forall a : A, is_adt (wrap a) = false) ->
+      {{ tenv }}
+        (Assign name (Const (match wrap w with SCA w => w | _ => W0 end)))
+      {{ [[`name ->> w as _]]::tenv }} ∪ {{ ext }} // env.
+  Proof.
+    intros * ? ? not_adt;
+      destruct (not_adt_is_sca not_adt) as (skol & Heq).
+    rewrite (Heq w) in *.
+    rewrite (TelEq_same_wrap _ (skol w)) by eauto.
+    apply CompileConstant; assumption.
+  Qed.
+
+  apply CompileConstant_SCA.
+  (* compile_constant value *)
+  compile_encoder_step.
+  compile_encoder_step.
+  compile_encoder_step.
+  compile_encoder_step.
+  compile_encoder_step.
+  compile_encoder_step.
+  compile_encoder_step.
+  compile_encoder_step.
+  compile_encoder_step.
+  compile_encoder_step.
+  compile_encoder_step.
+  compile_encoder_step.
+  compile_encoder_step.
+  compile_encoder_step.
+  compile_encoder_step.
+
+  rewrite encode_byte_simplify.
+  compile_encoder_step.
+  compile_encoder_step.
+  compile_encoder_step.
+  compile_encoder_step.
+  compile_encoder_step.
+  compile_encoder_step.
+  compile_encoder_step.
+
+  (* Add to properties *)
+  Lemma encode_word8_Impl_length :
+    forall (w: byte),
+      List.length (byteString (fst (encode_word_Impl w tt))) = 1.
+  Proof.
+    unfold encode_word_Impl; intros; rewrite encode_char'; reflexivity.
+  Qed.
+
+  Ltac _compile_decide_write8_side_condition ::=
+    repeat lazymatch goal with
+           | [ H := _ |- _ ] => unfold H in *; clear H
+           | [  |- context[List.length (byteString (?x))] ] =>
+             match x with
+             | transform_id => change (length (byteString transform_id)) with 0
+             | fst (EncodeBoundedNat _ _) => rewrite EncodeBoundedNat8_length
+             | fst (encode_word_Impl _ _) => rewrite encode_word8_Impl_length
+             | transform _ _ => rewrite ByteString_transform_length by _compile_decide_padding_0
+             | _ => fail 3 "Unrecognized form" x
+             end
+           | _ => omega
+           end.
+
+  Opaque encode_word_Impl.
+  compile_encoder_step.
+  compile_encoder_step.
+
+  Focus 3.
+  compile_encoder_step.
+  compile_encoder_step.
+  compile_encoder_step.
+  compile_encoder_step.
+  compile_encoder_step.
+  compile_encoder_step.
+  compile_encoder_step.
+  compile_encoder_step.
+  compile_encoder_step.
+  compile_encoder_step.
+  compile_encoder_step.
+  compile_encoder_step.
+  2: solve [compile_encoder_t].
+  2: solve [compile_encoder_t].
+  compile_encoder_step.
+  compile_encoder_step.
+  compile_encoder_step.
+  compile_encoder_step.
+  compile_encoder_step.
+  compile_encoder_step.
+  compile_encoder_step.
+  compile_encoder_step.
+  compile_encoder_step.
+  compile_encoder_step.
+  compile_encoder_step.
+  compile_encoder_step.
+  compile_encoder_step.
+  compile_encoder_step.
+  compile_encoder_step.
+  compile_encoder_step.
+  compile_encoder_step.
+  compile_encoder_step.
+
+  Transparent encode_word_Impl.
+  Lemma encode_word8_Impl_padding_0 : (* {cache} {cacheAddNat : CacheAdd cache nat} : *)
+    forall (w: byte), (* (c: @CacheEncode cache), *)
+      padding (fst (encode_word_Impl w tt)) = 0.
+  Proof.
+    unfold encode_word_Impl; intros; rewrite encode_char'; reflexivity.
+  Qed.
+  Opaque encode_word_Impl.
+
+  Ltac _compile_decide_padding_0 ::=
+  repeat first [ reflexivity |
+                 apply ByteString_transform_padding_0 |
+                 eapply encode_word8_Impl_padding_0 |
+                 eapply EncodeBoundedNat8_padding_0 ].
+
+  compile_encoder_step.
+
+  Focus 3.
+
+  compile_encoder_step.
+  compile_encoder_step.
+  compile_encoder_step.
+  compile_encoder_step.
+  compile_encoder_step.
+  compile_encoder_step.
+  compile_encoder_step.
+  compile_encoder_step.
+  compile_encoder_step.
+  compile_encoder_step.
+  compile_encoder_step.
+
+  compile_encoder_step.
+  compile_encoder_step.
+  2: solve [compile_encoder_t].
+  2: solve [compile_encoder_t].
+  compile_encoder_step.
+  compile_encoder_step.
+  compile_encoder_step.
+  compile_encoder_step.
+  compile_encoder_step.
+  compile_encoder_step.
+  compile_encoder_step.
+  compile_encoder_step.
+  compile_encoder_step.
+  compile_encoder_step.
+  compile_encoder_step.
+  compile_encoder_step.
+  compile_encoder_step.
+  compile_encoder_step.
+  compile_encoder_step.
+  compile_encoder_step.
+  compile_encoder_step.
+  compile_encoder_step.
+  compile_encoder_step.
+  compile_encoder_step.
+  compile_encoder_step.
+  compile_encoder_step.
+
+  Focus 3.
+  compile_encoder_step.
+  compile_encoder_step.
+  compile_encoder_step.
+  compile_encoder_step.
+  compile_encoder_step.
+  compile_encoder_step.
+  2:compile_encoder_t.
+
+Lemma CompileCallListSCALength {A}:
+  forall {WrpList: FacadeWrapper (Value ADTValue) (BoundedList A (pow2 8))}
+    (vlst varg : string) (tenv : Telescope ADTValue) (ext : StringMap.t (Value ADTValue))
+    env (lst : BoundedList A (pow2 8))
+    fLength tenv',
+    PreconditionSet tenv' ext [[[vlst;varg]]] ->
+    (exists sk: _ -> list W,
+        (forall ls: BoundedList A (pow2 8),
+            wrap ls = ADT (WordList (sk ls))) /\
+        (forall ls: BoundedList A (pow2 8),
+            List.length (sk ls) = List.length (`ls))) ->
+    GLabelMap.MapsTo fLength (Axiomatic WordListADTSpec.Length) env ->
+    TelEq ext tenv ([[`vlst ->> lst as _]]::tenv') -> (* Experiment to require a-posteriori reordering of variables *)
+    {{ tenv }}
+      Call varg fLength [vlst]
+    {{ [[ ` varg ->> BoundedListLength lst as _]]::tenv }} ∪ {{ ext }} // env.
+Proof.
+  intros * ? ? (? & wrap_eq & length_eq) ? Heq; setoid_rewrite Heq; PreconditionSet_t;
+  repeat (SameValues_Facade_t_step || facade_cleanup_call || LiftPropertyToTelescope_t || rewrite wrap_eq in *).
+  facade_eauto.
+  facade_eauto.
+  repeat match goal with
+         | [ H: ?a = ?a |- _ ] => clear dependent H
+         | [ H: ADT (WordList (_ _)) = ADT _ |- _ ] => inversion' H
+         end; rewrite length_eq; reflexivity.
+  facade_eauto.
+  rewrite remove_remove_comm by assumption; facade_eauto.
+Qed.
+
+Lemma CompileCallListBoundedNatLength:
+  forall (vlst varg : string) (tenv : Telescope ADTValue) (ext : StringMap.t (Value ADTValue))
+    env (lst : BoundedList (BoundedNat 8) (pow2 8))
+    fLength tenv',
+    PreconditionSet tenv' ext [[[vlst;varg]]] ->
+    GLabelMap.MapsTo fLength (Axiomatic WordListADTSpec.Length) env ->
+    TelEq ext tenv ([[`vlst ->> lst as _]]::tenv') -> (* Experiment to require a-posteriori reordering of variables *)
+    {{ tenv }}
+      Call varg fLength [vlst]
+    {{ [[ ` varg ->> BoundedListLength lst as _]]::tenv }} ∪ {{ ext }} // env.
+Proof.
+  intros.
+  eapply CompileCallListSCALength; eauto.
+  eexists; split.
+  - reflexivity.
+  - setoid_rewrite map_length; reflexivity.
+Qed.
+
+
+Ltac _compile_CallListLength ::=
+  match_ProgOk
+    ltac:(fun _ _ post _ _ =>
+            match post with
+            | [[ _ ->> BoundedListLength ?lst as _]] :: _ =>
+              let vlst := find_name_in_precondition lst in
+              (* FIXME use this instead of explicit continuations in every lemma *)
+              compile_do_use_transitivity_to_handle_head_separately;
+              [ eapply (CompileCallListBoundedNatLength vlst) | ]
+            end).
+
+  compile_encoder_step.
+  3: compile_encoder_step.
+  compile_encoder_step.
+  compile_encoder_step.
+  compile_encoder_step.
+  compile_encoder_step.
+  compile_encoder_step.
+  compile_encoder_step.
+  compile_encoder_step.
+  compile_encoder_step.
+  compile_encoder_step.
+  compile_encoder_step.
+  2:compile_encoder_step.
+  2:compile_encoder_step.
+
+
 
 Record BitArrayAndList :=
   { f1 : BitArray 8;
@@ -151,28 +574,6 @@ Definition BitArrayAndListAsCollectionOfVariables
 Hint Unfold BitArrayAndList_encode : f2f_binencoders_autorewrite_db.
 Hint Unfold BitArrayAndListAsCollectionOfVariables : f2f_binencoders_autorewrite_db.
 Hint Rewrite (@IList_encode'_body_simpl empty_cache) : f2f_binencoders_autorewrite_db.
-
-Typeclasses eauto := 10.
-
-Instance WrapListOfBoundedValues :
-  (* FIXME when the elements of the list inject into W, we should have a
-     canonical into lists of words. *)
-  FacadeWrapper (Value ADTValue) (list (BoundedN 8)). Admitted.
-
-Lemma map_inj {A B}:
-  forall (f: A -> B),
-    (forall x y, f x = f y -> x = y) ->
-    (forall x y, (map f) x = (map f) y -> x = y).
-Proof.
-  induction x; destruct y; simpl; intros HH; try congruence.
-  inversion' HH; f_equal; eauto.
-Qed.
-
-Instance WrapList {A B} {Wrp: FacadeWrapper A B} : FacadeWrapper (list A) (list B).
-Proof.
-  refine {| wrap x := map wrap x |}.
-  eauto using map_inj, wrap_inj.
-Qed.
 
 Example BitArrayAndList_compile :
   ParametricExtraction
